experiments: simplifying invariants for map

case_studies/tests/src/iterator.rs
@@ -1,0 +1,11 @@
+
+
+#[rr::returns("seqZ 0 10")]
+fn test_iterator_1() -> Vec<i32> {
+    (0..10).collect()
+}
+
+#[rr::returns("seqZ 0 10")]
+fn test_iterator_2() -> Vec<i32> {
+    (0..10).map(#[rr::returns("x")] |x| x).collect()
+}
