stdlib/iterator/theories/map.v
@@ -1,5 +1,6 @@
 From refinedrust Require Import typing shims.
 From rrstd.iterator.theories Require Import iterator.
+From rrstd.closures.closures.generated Require Import generated_specs_closures.
 
 Record MapX (I : RT) (F : RT) : Type := mk_map_x {
   map_it : RT_xt I;
@@ -47,15 +48,90 @@ Proof.
   unfold li_sealed. iIntros "#Ha". iModIntro. done.
 Qed.
 
+Section closure_props.
+  Context `{!refinedrustGS Σ}.
+
+  Context (Clos_rt Args_rt Clos_out_rt : RT).
+
+  Class ClosureHasTrivialPre (fnonce_attrs : FnOnce_spec_attrs Clos_rt Args_rt Clos_out_rt) := closure_has_trivial_pre_proof : ∀ π self args, ⊢ FnOnce_Pre fnonce_attrs π self args.
+
+End closure_props.
+
+Ltac solve_closure_has_trivial_pre :=
+  match goal with
+  | |- ClosureHasTrivialPre _ _ _ _ =>
+    unfold ClosureHasTrivialPre;
+    intros ???; prepare_initial_coq_context;
+    iStartProof;
+    unshelve (repeat liRStep; solve[fail]);
+    unshelve (sidecond_solver);
+    sidecond_hammer; 
+    apply inhabitant
+  end.
+
+(* TODO: don't have this as hint, but generate instances in the frontend *)
+Global Hint Extern 100 (ClosureHasTrivialPre _ _ _ _) =>
+  solve_closure_has_trivial_pre : typeclass_instances.
+
+Section map_inv_variants.
+  Context `{!refinedrustGS Σ}.
+
+  Definition map_inv_ty (Self_rt Item_rt Clos_rt Clos_out_rt : RT)
+    (fnonce_attrs : FnOnce_spec_attrs Clos_rt (tuple1_rt Item_rt) Clos_out_rt)
+    (fnmut_attrs : FnMut_spec_attrs Clos_rt (tuple1_rt Item_rt) Clos_out_rt) :=
+    thread_id → RT_xt Self_rt → RT_xt Clos_rt → iProp Σ.
+  Global Arguments map_inv_ty : simpl never.
+
+  Context
+    (Self_rt Item_rt Clos_rt Clos_out_rt : RT)
+    (fnonce_attrs : FnOnce_spec_attrs Clos_rt (tuple1_rt Item_rt) Clos_out_rt)
+    (fnmut_attrs : FnMut_spec_attrs Clos_rt (tuple1_rt Item_rt) Clos_out_rt)
+  .
+
+  Lemma simpl_exist_map_inv_trivial Q :
+    SimplExist (map_inv_ty _ _ _ _ fnonce_attrs fnmut_attrs) Q
+      (∃ (Inv : thread_id → RT_xt Self_rt → RT_xt Clos_rt → iProp Σ), Q Inv).
+  Proof.
+    unfold SimplExist.
+    done.
+  Qed.
+
+  (* For a trivial pre, instantiate with a trivial invariant *)
+  Lemma simpl_exist_map_inv_pure_pre Q :
+    ClosureHasTrivialPre _ _ _ fnonce_attrs →
+    SimplExist (map_inv_ty Self_rt Item_rt Clos_rt Clos_out_rt fnonce_attrs fnmut_attrs) Q
+      (Q (λ _ _ _, True)%I).
+  Proof.
+    intros Hpre.
+    unfold SimplExist.
+    eauto with iFrame.
+  Qed.
+
+  Lemma simpl_forall_map_inv Q :
+    SimplForall (map_inv_ty _ _ _ _ fnonce_attrs fnmut_attrs) 1 Q (∀ (Inv : thread_id → RT_xt Self_rt → RT_xt Clos_rt → iProp Σ), Q Inv).
+  Proof.
+    unfold SimplForall.
+    done.
+  Qed.
+End map_inv_variants.
+Global Hint Extern 1000 (SimplExist (map_inv_ty _ _ _ _ ?fnonce ?fnmut) _ _) =>
+  notypeclasses refine (simpl_exist_map_inv_trivial _ _ _ _ fnonce fnmut _) : typeclass_instances.
+Global Hint Extern 10 (SimplForall (map_inv_ty _ _ _ _ ?fnonce ?fnmut) _ _ _) =>
+  notypeclasses refine (simpl_forall_map_inv _ _ _ _ fnonce fnmut _) : typeclass_instances.
+
+Global Hint Extern 100 (SimplExist (map_inv_ty _ _ _ _ ?fnonce ?fnmut) _ _) =>
+  notypeclasses refine (simpl_exist_map_inv_pure_pre _ _ _ _ fnonce fnmut _ _);
+  typeclasses eauto : typeclass_instances.
+
 Section map.
   Context `{RRGS : !refinedrustGS Σ}.
-  Definition MapInv {Self_rt Item_rt Clos_rt Clos_out_rt : RT} 
+  Definition MapInv {Self_rt Item_rt Clos_rt Clos_out_rt : RT}
     (iter_attrs : traits_iterator_Iterator_spec_attrs Self_rt Item_rt)
     (Pre : thread_id → RT_xt Clos_rt → RT_xt (tuple1_rt Item_rt) → iProp Σ)
-    (PostMut : thread_id → RT_xt Clos_rt → RT_xt (tuple1_rt Item_rt) → RT_xt Clos_rt → RT_xt Clos_out_rt → iProp Σ) 
+    (PostMut : thread_id → RT_xt Clos_rt → RT_xt (tuple1_rt Item_rt) → RT_xt Clos_rt → RT_xt Clos_out_rt → iProp Σ)
     (*(fnonce_attrs : FnOnce_spec_attrs Clos_rt (tuple1_rt Item_rt) Clos_out_rt)*)
     (*(fnmut_attrs : FnMut_spec_attrs Clos_rt (tuple1_rt Item_rt) Clos_out_rt) *)
-    : _ → _ → iProp Σ := 
+    : _ → _ → iProp Σ :=
     λ (π : thread_id) (s : MapX Self_rt Clos_rt),
     (∃ (Inv : thread_id → RT_xt Self_rt → RT_xt Clos_rt → iProp Σ),
       (* user-picked invariant *)
@@ -67,7 +143,7 @@ Section map.
         (☒ iter_attrs.(traits_iterator_Iterator_Next) π it_state (Some e) it_state') -∗
         Inv π it_state clos_state -∗
         Pre π clos_state *[e] ∗
-        (∀ e' clos_state', PostMut π clos_state *[e] clos_state' e' -∗ Inv π it_state' clos_state'))) ∗
+        (∀ e' clos_state', ☒ PostMut π clos_state *[e] clos_state' e' -∗ Inv π it_state' clos_state'))) ∗
       (* progress (no element) *)
       li_sealed (□ (∀ it_state it_state' clos_state,
         (☒ iter_attrs.(traits_iterator_Iterator_Next) π it_state None it_state') -∗
